---
id: 1469147828941434881
author:artistexyz
published_date:{{PUBLISHED_DATE }}
conversation_id: Conversation-1468687643214958595
in_reply_to: 1469011745029214209
retweet: None
quoted_tweet: None
---

@yudapearl Okay. 8hrs later, I figured it out. ACE=PNS if monotonicity. In general
ACE= P(y_0=0, y_1=1)-P(y_0=1, y_1=0)
monotonicity implies second term is zero, and first term is PNS

### Metadata

Author: [[@artistexyz]]
Conversation: [[Conversation-1468687643214958595]]
In reply to: [[1469011745029214209]]
Retweet of: [[None]]
Quoted tweet: [[None]]
