---
id: 1484763488878690306
author:yudapearl
published_date:{{PUBLISHED_DATE }}
conversation_id: Conversation-1484707033291001858
in_reply_to: 1484730766508630020
retweet: None
quoted_tweet: None
---

@artistexyz Here is a simple derivation of ETT=P(y_0=1|x=1)
The key is to write P(y_0=1) =P(y=1|do(x=0) as
P(y_0=1) = P(y_0=1| x=1) P(x=1) + 
                   P(y_0=1|x=0)P(x=0)
            = ETT P(x=1) + P(y=1|X=0)(1-P(x=1)
This gives ETT in terms of L1 and L2 probabilities.

### Metadata

Author: [[@yudapearl]]
Conversation: [[Conversation-1484707033291001858]]
In reply to: [[1484730766508630020]]
Retweet of: [[None]]
Quoted tweet: [[None]]
